theories/monotone.v
@@ -30,51 +30,59 @@ Section monotone.
       apply std_rel_pub_rtc_Permanent in Hrelated; subst; auto.
     - destruct Hrelated as [ [Hdom_sta Hrelated] _]. simpl in *.
       assert (is_Some (W'.1 !! a)) as [y Hy].
-      { rewrite -elem_of_dom. apply elem_of_subseteq in Hdom_sta. apply Hdom_sta. rewrite elem_of_dom.
-        eauto. }
-      specialize (Hrelated _ Permanent y Hstate Hy).
-      apply std_rel_pub_rtc_Permanent in Hrelated; subst; auto.
+      { rewrite -elem_of_dom. apply elem_of_subseteq in Hdom_sta.
+        apply Hdom_sta. rewrite elem_of_dom.
+        destruct Hstate ; eauto.
+      }
+      destruct Hstate as [Hstate|Hstate].
+      + specialize (Hrelated _ Permanent y Hstate Hy).
+        apply std_rel_pub_rtc_Permanent in Hrelated; subst; auto.
+      + specialize (Hrelated _ Temporary y Hstate Hy).
+        apply std_rel_pub_rtc_Temporary in Hrelated; subst; auto.
   Qed.
 
-  Lemma region_state_nwl_monotone_a W W' (a a' : Addr) l :
-    (a < a')%a →
-    related_sts_a_world W W' a' →
-    region_state_nwl W a l -> region_state_nwl W' a l.
-  Proof.
-    rewrite /region_state_nwl /std.
-    intros Hlt Hrelated Hstate.
-    destruct l.
-    - destruct Hrelated as [ [Hdom_sta Hrelated ] _]. simpl in *.
-      assert (is_Some (W'.1 !! a)) as [y Hy].
-      { rewrite -elem_of_dom. apply elem_of_subseteq in Hdom_sta. apply Hdom_sta. rewrite elem_of_dom;eauto. }
-      specialize (Hrelated a Permanent y Hstate Hy).
-      eapply rtc_implies in Hrelated.
-      apply std_rel_pub_plus_rtc_Permanent in Hrelated; subst; auto.
-      intros r q. destruct (decide (a' <= a)%a);auto.
-    - destruct Hrelated as [ [Hdom_sta Hrelated] _]. simpl in *.
-      assert (is_Some (W'.1 !! a)) as [y Hy].
-      { rewrite -elem_of_dom. apply elem_of_subseteq in Hdom_sta. apply Hdom_sta. rewrite elem_of_dom.
-        eauto. }
-      specialize (Hrelated _ Permanent y Hstate Hy).
-      eapply rtc_implies in Hrelated.
-      apply std_rel_pub_plus_rtc_Permanent in Hrelated; subst; auto.
-      intros r q. destruct (decide (a' <= a)%a);auto.
-  Qed.
+  (* Lemma region_state_nwl_monotone_a W W' (a a' : Addr) l : *)
+  (*   (a < a')%a → *)
+  (*   related_sts_a_world W W' a' → *)
+  (*   region_state_nwl W a l -> region_state_nwl W' a l. *)
+  (* Proof. *)
+  (*   rewrite /region_state_nwl /std. *)
+  (*   intros Hlt Hrelated Hstate. *)
+  (*   destruct l. *)
+  (*   - destruct Hrelated as [ [Hdom_sta Hrelated ] _]. simpl in *. *)
+  (*     assert (is_Some (W'.1 !! a)) as [y Hy]. *)
+  (*     { rewrite -elem_of_dom. apply elem_of_subseteq in Hdom_sta. apply Hdom_sta. rewrite elem_of_dom;eauto. } *)
+  (*     specialize (Hrelated a Permanent y Hstate Hy). *)
+  (*     eapply rtc_implies in Hrelated. *)
+  (*     apply std_rel_pub_plus_rtc_Permanent in Hrelated; subst; auto. *)
+  (*     intros r q. destruct (decide (a' <= a)%a);auto. *)
+  (*   - destruct Hrelated as [ [Hdom_sta Hrelated] _]. simpl in *. *)
+  (*     assert (is_Some (W'.1 !! a)) as [y Hy]. *)
+  (*     { rewrite -elem_of_dom. apply elem_of_subseteq in Hdom_sta. *)
+  (*       apply Hdom_sta. rewrite elem_of_dom. *)
+  (*       destruct Hstate ; eauto. *)
+  (*     } *)
+  (*     destruct Hstate as [Hstate|Hstate]. *)
+  (*     + specialize (Hrelated _ Permanent y Hstate Hy). *)
+  (*       apply std_rel_pub_rtc_Permanent in Hrelated; subst; auto. *)
+  (*     + specialize (Hrelated _ Temporary y Hstate Hy). *)
+  (*       apply std_rel_pub_rtc_Temporary in Hrelated; subst; auto. *)
+  (* Qed. *)
 
-  Lemma region_state_nwl_monotone_nm W W' a :
-    related_sts_priv_world W W' →
-    region_state_nwl W a Local -> region_state_nwl W' a Local.
-  Proof.
-    rewrite /region_state_nwl /std.
-    intros Hrelated Hstate.
-    destruct Hrelated as [ [Hdom_sta Hrelated ] _].
-    assert (is_Some (W'.1 !! a)) as [y Hy].
-    { rewrite -elem_of_dom. apply elem_of_subseteq in Hdom_sta. apply Hdom_sta. rewrite elem_of_dom;eauto. }
-    specialize (Hrelated _ Permanent y Hstate Hy).
-    apply std_rel_rtc_Permanent in Hrelated; subst; auto.
-  Qed.
+  (* Lemma region_state_nwl_monotone_nm W W' a : *)
+  (*   related_sts_priv_world W W' → *)
+  (*   region_state_nwl W a Local -> region_state_nwl W' a Local. *)
+  (* Proof. *)
+  (*   rewrite /region_state_nwl /std. *)
+  (*   intros Hrelated Hstate. *)
+  (*   destruct Hrelated as [ [Hdom_sta Hrelated ] _]. *)
+  (*   assert (is_Some (W'.1 !! a)) as [y Hy]. *)
+  (*   { rewrite -elem_of_dom. apply elem_of_subseteq in Hdom_sta. apply Hdom_sta. rewrite elem_of_dom;eauto. } *)
+  (*   specialize (Hrelated _ Permanent y Hstate Hy). *)
+  (*   apply std_rel_rtc_Permanent in Hrelated; subst; auto. *)
+  (* Qed. *)
 
-  Lemma region_state_nwl_monotone_nm_nl W W' a :
+  Lemma region_state_nwl_monotone_nl W W' a :
     related_sts_priv_world W W' →
     region_state_nwl W a Global -> region_state_nwl W' a Global.
   Proof.
@@ -87,7 +95,7 @@ Section monotone.
     apply std_rel_rtc_Permanent in Hrelated; subst; auto.
   Qed.
 
-  Lemma region_state_pwl_monotone_mono W W' a :
+  Lemma region_state_pwl_monotone W W' a :
     related_sts_pub_world W W' →
     region_state_pwl W a -> region_state_pwl W' a.
   Proof.
@@ -100,21 +108,21 @@ Section monotone.
     apply std_rel_pub_rtc_Temporary in Hrelated; subst; auto.
   Qed.
 
-  Lemma region_state_pwl_monotone_a W W' a a' :
-    (a < a')%a →
-    related_sts_a_world W W' a' →
-    region_state_pwl W a -> region_state_pwl W' a.
-  Proof.
-    rewrite /region_state_pwl /std.
-    intros Hle Hrelated Hstate.
-    destruct Hrelated as [ [Hdom_sta Hrelated ] _]. simpl in *.
-    assert (is_Some (W'.1 !! a)) as [y Hy].
-    { rewrite -elem_of_dom. apply elem_of_subseteq in Hdom_sta. apply Hdom_sta. rewrite elem_of_dom;eauto. }
-    specialize (Hrelated _ Temporary y Hstate Hy).
-    eapply rtc_implies in Hrelated.
-    apply std_rel_pub_rtc_Temporary in Hrelated; subst; auto.
-    intros r q. rewrite decide_False;auto. solve_addr.
-  Qed.
+  (* Lemma region_state_pwl_monotone_a W W' a a' : *)
+  (*   (a < a')%a → *)
+  (*   related_sts_a_world W W' a' → *)
+  (*   region_state_pwl W a -> region_state_pwl W' a. *)
+  (* Proof. *)
+  (*   rewrite /region_state_pwl /std. *)
+  (*   intros Hle Hrelated Hstate. *)
+  (*   destruct Hrelated as [ [Hdom_sta Hrelated ] _]. simpl in *. *)
+  (*   assert (is_Some (W'.1 !! a)) as [y Hy]. *)
+  (*   { rewrite -elem_of_dom. apply elem_of_subseteq in Hdom_sta. apply Hdom_sta. rewrite elem_of_dom;eauto. } *)
+  (*   specialize (Hrelated _ Temporary y Hstate Hy). *)
+  (*   eapply rtc_implies in Hrelated. *)
+  (*   apply std_rel_pub_rtc_Temporary in Hrelated; subst; auto. *)
+  (*   intros r q. rewrite decide_False;auto. solve_addr. *)
+  (* Qed. *)
 
   (* Lemma region_state_nwl_future W W' l l' p a a': *)
   (*   (a < a')%a → *)
@@ -283,7 +291,7 @@ Section monotone.
       iApply (big_sepL_mono with "Hw").
       iIntros (n y Hsome) "Hw".
       iDestruct "Hw" as (p) "(%Hflow & Hrw & %Hrel)".
-      eapply region_state_pwl_monotone_mono in Hrel;auto.
+      eapply region_state_pwl_monotone in Hrel;auto.
     - iApply (big_sepL_mono with "Hw").
       iIntros (n y Hsome) "Hw".
       iDestruct "Hw" as (P Hpers) "#[Hrw Hrel]".
@@ -299,7 +307,7 @@ Section monotone.
         iApply "Hw".
       + iIntros (Hrelated').
         iAssert (future_world Local W W'')%I as "Hrelated".
-        { iPureIntro. apply related_sts_pub_priv_trans_world with W'; auto. }
+        { iPureIntro. apply related_sts_pub_trans_world with W'; auto. }
         iSpecialize ("Hw" $! r W'' with "Hrelated").
         iApply "Hw".
     - iApply (big_sepL_mono with "Hw").
@@ -312,7 +320,7 @@ Section monotone.
       iApply (big_sepL_mono with "Hw").
       iIntros (n y Hsome) "Hw".
       iDestruct "Hw" as (p) "(%Hflow & Hrw & %Hrel)".
-      eapply region_state_pwl_monotone_mono in Hrel;auto.
+      eapply region_state_pwl_monotone in Hrel;auto.
   Qed.
 
   (* Definition aOf (w : Word) : Addr := *)
@@ -322,55 +330,53 @@ Section monotone.
   (*   end. *)
 
   (* Lemma interp_monotone_a W W' w : *)
-  (*   ⌜related_sts_a_world W W' (aOf w)⌝ -∗ *)
+  (*   ⌜related_sts_pub_world W W'⌝ -∗ *)
   (*   interp W w -∗ interp W' w. *)
   (* Proof. *)
   (*   iIntros (Hrelated) "#Hw". *)
   (*   rewrite /interp /= fixpoint_interp1_eq /=. *)
   (*   destruct w; rewrite fixpoint_interp1_eq /=; auto. *)
-  (*   destruct c,p,p,p,p; auto; simpl in Hrelated. *)
+  (*   destruct sb,p; auto; simpl in Hrelated. *)
   (*   - iApply (big_sepL_mono with "Hw"). *)
   (*     iIntros (n y Hsome) "Hw". *)
   (*     iDestruct "Hw" as (P Hpers) "#[Hrw Hrel]". *)
   (*     iExists _. iSplit;eauto. iFrame "#". *)
   (*     iDestruct "Hrel" as %Hrel. *)
-  (*     iPureIntro. apply region_state_nwl_monotone_a with W a0;auto. *)
-  (*     eapply region_addrs_lookup_le;eauto. *)
+  (*     iPureIntro. apply region_state_nwl_monotone with W;auto. *)
   (*   - iApply (big_sepL_mono with "Hw"). *)
   (*     iIntros (n y Hsome) "Hw". *)
   (*     iDestruct "Hw" as "#[Hrw Hrel]". *)
   (*     iSplit;eauto. iFrame "#". *)
   (*     iDestruct "Hrel" as %Hrel. *)
-  (*     iPureIntro. apply region_state_nwl_monotone_a with W a0;auto. eapply region_addrs_lookup_le;eauto.  *)
-  (*   - destruct l; auto. *)
+  (*     iPureIntro. apply region_state_nwl_monotone with W;auto. *)
+  (*   - destruct g; auto. *)
   (*     iApply (big_sepL_mono with "Hw"). *)
   (*     iIntros (n y Hsome) "Hw". *)
-  (*     iDestruct "Hw" as "#[Hrw Hrel]". *)
-  (*     iSplit;eauto. iFrame "#". *)
+  (*     iDestruct "Hw" as (p' Hfl) "#[Hrw Hrel]". *)
+  (*     iExists _. iSplit;eauto. iFrame "#". *)
   (*     iDestruct "Hrel" as %Hrel. *)
-  (*     iPureIntro. *)
-  (*     apply region_state_pwl_monotone_a with W a0;auto. eapply region_addrs_lookup_le;eauto.  *)
+  (*     iPureIntro. apply region_state_pwl_monotone with W;auto. *)
   (*   - iApply (big_sepL_mono with "Hw"). *)
   (*     iIntros (n y Hsome) "Hw". *)
   (*     iDestruct "Hw" as (P Hpers) "#[Hrw Hrel]". *)
   (*     iExists _. iSplit;eauto. iFrame "#". *)
   (*     iDestruct "Hrel" as %Hrel. *)
-  (*     iPureIntro. apply region_state_nwl_monotone_a with W a0;auto. eapply region_addrs_lookup_le;eauto.  *)
+  (*     iPureIntro. apply region_state_nwl_monotone with W a0;auto. eapply region_addrs_lookup_le;eauto. *)
   (*   - iModIntro. iIntros (r W''). *)
   (*     destruct l; simpl. *)
   (*     + iIntros (Hrelated'). *)
   (*       iAssert (future_world Global a W W'')%I as "Hrelated". *)
-  (*       { iPureIntro. apply related_sts_a_priv_trans_world with W' a0; auto. } *)
+  (*       { iPureIntro. apply related_sts_priv_trans_world with W' a0; auto. } *)
   (*       iSpecialize ("Hw" $! r W'' with "Hrelated"). *)
   (*       iApply "Hw". *)
   (*     + iIntros (Hrelated'). *)
   (*       iAssert (future_world Local a W W'')%I as "Hrelated". *)
-  (*       { iPureIntro. apply related_sts_a_priv_trans_world with W' a0; auto. } *)
+  (*       { iPureIntro. apply related_sts_priv_trans_world with W' a0; auto. } *)
   (*       iSpecialize ("Hw" $! r W'' with "Hrelated"). *)
   (*       iApply "Hw". *)
   (*     + iIntros (Hrelated'). *)
   (*       iAssert (future_world Directed a0 W W'')%I as "Hrelated". *)
-  (*       { iPureIntro. apply related_sts_a_trans_world with W';auto. } *)
+  (*       { iPureIntro. apply related_sts_trans_world with W';auto. } *)
   (*       iSpecialize ("Hw" $! r W'' with "Hrelated"). *)
   (*       iApply "Hw". *)
   (*   - iApply (big_sepL_mono with "Hw"). *)
@@ -378,14 +384,14 @@ Section monotone.
   (*     iDestruct "Hw" as "#[Hrw Hrel]". *)
   (*     iSplit;eauto. iFrame "#". *)
   (*     iDestruct "Hrel" as %Hrel. *)
-  (*     iPureIntro. apply region_state_nwl_monotone_a with W a0;auto. eapply region_addrs_lookup_le;eauto.  *)
+  (*     iPureIntro. apply region_state_nwl_monotone with W a0;auto. eapply region_addrs_lookup_le;eauto. *)
   (*   - destruct l; auto. *)
   (*     iApply (big_sepL_mono with "Hw"). *)
   (*     iIntros (n y Hsome) "Hw". *)
   (*     iDestruct "Hw" as "#[Hrw Hrel]". *)
   (*     iSplit;eauto. iFrame "#". *)
   (*     iDestruct "Hrel" as %Hrel. *)
-  (*     iPureIntro. apply region_state_pwl_monotone_a with W a0;auto. eapply region_addrs_lookup_le;eauto.  *)
+  (*     iPureIntro. apply region_state_pwl_monotone with W a0;auto. eapply region_addrs_lookup_le;eauto. *)
   (*   - destruct l; simpl. *)
   (*     + iApply (big_sepL_mono with "Hw"). *)
   (*       iIntros (n y Hsome) "Hw". *)
@@ -393,7 +399,7 @@ Section monotone.
   (*       iSplit;eauto. iFrame "#". *)
   (*       iDestruct "Hst" as %Hst. *)
   (*       iPureIntro. apply region_state_nwl_monotone_nm_nl with W;auto. *)
-  (*       apply related_sts_pub_plus_priv_world, related_sts_a_pub_plus_world with a;auto.  *)
+  (*       apply related_sts_pub_plus_priv_world, related_sts_pub_plus_world with a;auto. *)
   (*     + iDestruct "Hw" as "[Hw1 Hw2]". *)
   (*       iSplitL "Hw1". *)
   (*       * iApply (big_sepL_mono with "Hw1"). *)
@@ -401,8 +407,8 @@ Section monotone.
   (*         iDestruct "Hw" as "#[Hrw Hst ]". *)
   (*         iSplit;eauto. iFrame "#". *)
   (*         iDestruct "Hst" as %Hstd. *)
-  (*         iPureIntro. eapply (region_state_nwl_monotone_a W W' _ (addr_reg.min a a0) Local); auto. *)
-  (*         eapply region_addrs_lookup_le;eauto.  apply related_sts_a_weak_world with a;auto. solve_addr.  *)
+  (*         iPureIntro. eapply (region_state_nwl_monotone W W' _ (addr_reg.min a a0) Local); auto. *)
+  (*         eapply region_addrs_lookup_le;eauto.  apply related_sts_a_weak_world with a;auto. solve_addr. *)
   (*       * iApply (big_sepL_mono with "Hw2"). *)
   (*         iIntros (n y Hsome) "Hw". *)
   (*         iDestruct "Hw" as "#[Hrw Hst ]". *)
@@ -625,7 +631,7 @@ Section monotone.
   (*   - destruct l; try discriminate. done. done. *)
   (* Qed. *)
 
- Lemma interp_monotone_nm_nl W W' w :
+ Lemma interp_monotone_nl W W' w :
     ⌜related_sts_priv_world W W'⌝ -∗ ⌜isLocalWord w = false⌝ -∗
     interp W w -∗ interp W' w.
   Proof.
@@ -639,7 +645,7 @@ Section monotone.
       iExists _. iSplit;eauto. iFrame "#".
       iDestruct "Hrel" as %Hrel.
       iPureIntro. destruct g; try discriminate.
-      apply region_state_nwl_monotone_nm_nl with W;auto.
+      apply region_state_nwl_monotone_nl with W;auto.
     - iApply (big_sepL_mono with "Hw").
       iIntros (n y Hsome) "Hw".
       iDestruct "Hw" as "#[Hrw Hrel ]".
@@ -647,7 +653,7 @@ Section monotone.
       iSplit;eauto. iFrame "#".
       iDestruct "Hrel" as %Hrel.
       iPureIntro. destruct g; try discriminate.
-      apply region_state_nwl_monotone_nm_nl with W;auto.
+      apply region_state_nwl_monotone_nl with W;auto.
     - destruct g; auto. discriminate.
     - iApply (big_sepL_mono with "Hw").
       iIntros (n y Hsome) "Hw".
@@ -655,7 +661,7 @@ Section monotone.
       iExists _. iSplit;eauto. iFrame "#".
       iDestruct "Hrel" as %Hrel.
       iPureIntro. destruct g; try discriminate.
-      apply region_state_nwl_monotone_nm_nl with W;auto.
+      apply region_state_nwl_monotone_nl with W;auto.
     - iModIntro. iIntros (r W'').
       destruct g; simpl; try discriminate.
       iIntros (Hrelated').
@@ -669,14 +675,14 @@ Section monotone.
       iSplit;eauto. iFrame "#".
       iDestruct "Hrel" as %Hrel.
       iPureIntro. destruct g; try discriminate.
-      apply region_state_nwl_monotone_nm_nl with W;auto.
+      apply region_state_nwl_monotone_nl with W;auto.
     - destruct g; try discriminate. done.
   Qed.
 
   (*Lemma that allows switching between the two different formulations of monotonicity, to alleviate the effects of inconsistencies*)
-  Lemma switch_monotonicity_formulation ρ l w φ:
+  Lemma switch_monotonicity_formulation ρ w φ:
       ρ ≠ Revoked → (∀ m, ρ ≠ Frozen m) ->
-      monotonicity_guarantees_region ρ l w φ ≡ monotonicity_guarantees_decide (Σ := Σ) ρ l w φ.
+      monotonicity_guarantees_region ρ w φ ≡ monotonicity_guarantees_decide (Σ := Σ) ρ w φ.
   Proof.
     intros Hrev Hmono.
     unfold monotonicity_guarantees_region, monotonicity_guarantees_decide.
@@ -700,7 +706,7 @@ Section monotone.
     iFrame.
     iDestruct "Hperm" as %Hperm.
     iPureIntro.
-    apply (region_state_nwl_monotone_nm_nl _ W') in Hperm; auto.
+    apply (region_state_nwl_monotone_nl _ W') in Hperm; auto.
   Qed.
 
   Lemma adv_stack_monotone W W' b e :
@@ -715,7 +721,7 @@ Section monotone.
     iIntros (k y Hsome) "(Hr & Htemp)".
     iDestruct "Htemp" as %Htemp.
     iFrame. iPureIntro.
-    apply (region_state_pwl_monotone_mono _ W') in Htemp; auto.
+    apply (region_state_pwl_monotone _ W') in Htemp; auto.
   Qed.
 
   Global Instance interp_ne n :
@@ -731,35 +737,58 @@ Lemma interp_monotone_generalW (W : WORLD)  (ρ : region_type) (p p0 : Perm) (l 
   withinBounds a2 a1 a0 = true →
   canStore p0 (WCap p g b e a) = true →
   ((fixpoint interp1) W) (WCap p0 l a2 a1 a0) -∗
-  monotonicity_guarantees_region ρ a0 (WCap p g b e a) (λne Wv : WORLD * (leibnizO Word), (interp Wv.1) Wv.2).
+  monotonicity_guarantees_region ρ (WCap p g b e a) (λne Wv : WORLD * (leibnizO Word), (interp Wv.1) Wv.2).
 Proof.
+
+  unfold monotonicity_guarantees_region.
+  iIntros (Hstd Hwb Hconds) "#Hvdst".
+  destruct ρ.
+  - destruct (pwl p0) eqn: HpwlP1 ; iAlways; simpl.
+    * iIntros (W0 W1) "% HIW0".
+        iApply interp_monotone;eauto.
+    * iIntros (W0 W1) "% HIW0".
+      destruct g.
+    + iApply interp_monotone_nl; eauto.
+    (*The below case is a contradiction, since if g is local,p0 must be WL and p0 flows into the non-WL p1*)
+    + destruct p0 ; try (simpl in Hconds; by exfalso).
+      all:destruct p1 eqn:Hp1v ; (by exfalso).
+  - iAlways. simpl. iIntros (W0 W1) "% HIW0".
+    destruct g.
+    + by iApply interp_monotone_nl.
+    + (*Trick here: value relation leads to a contradiction if p0 is WL, since then its region cannot be permanent*)
+      iDestruct ( writeLocalAllowed_valid_cap_implies with "Hvdst" ) as %Ha; eauto.
+      rewrite Hstd in Ha. inversion Ha.
+  - auto.
+  - auto.
+
+
   unfold monotonicity_guarantees_region.
   iIntros (Hstd Hwb Hconds) "#Hvdst".
   destruct ρ;auto.
   - iModIntro; simpl;auto.
     iIntros (W0 W1) "%Hrel HIW0".
     destruct g.
-    * iApply (interp_monotone_nm_nl with "[] [] HIW0");auto.
+    * iApply (interp_monotone_nl with "[] [] HIW0");auto.
       iPureIntro.
       apply related_sts_a_pub_plus_world in Hrel.
       apply related_sts_pub_plus_priv_world;auto.
-    * admit.
-    (* * iApply (interp_monotone_nm_nl with "[] [] HIW0");auto. *)
-    (*   iPureIntro. apply related_sts_pub_plus_priv_world. apply related_sts_a_pub_plus_world with a0;auto. *)
-    (* * destruct (decide (p = O)). *)
-    (*   { subst. rewrite !fixpoint_interp1_eq. done. } *)
-    (*   iApply (interp_monotone_a with "[] HIW0");auto. *)
-    (*   apply andb_prop in Hconds as [Hp0 Hleb]. *)
-    (*   simpl. destruct (isU p) eqn:Hu. *)
-    (*   ** assert (a <= a0)%a as Hle. *)
-    (*      { destruct p; inversion Hu;simpl in Hleb;apply Z.leb_le in Hleb;solve_addr. } *)
-  (*      iPureIntro. apply related_sts_a_weak_world with a0;auto. *)
-    (*   ** assert (e <= a0)%a as Hle. *)
-    (*      { destruct p; inversion Hu;simpl in Hleb;apply Z.leb_le in Hleb; try solve_addr. } *)
-    (*      iPureIntro. apply related_sts_a_weak_world with a0;auto. *)
+    * iApply (interp_monotone with "[] [] HIW0");auto.
+      iPureIntro. apply related_sts_pub_plus_priv_world.
+      eapply related_sts_pub_world;auto.
+    * destruct (decide (p = O)).
+      { subst. rewrite !fixpoint_interp1_eq. done. }
+      iApply (interp_monotone_a with "[] HIW0");auto.
+      apply andb_prop in Hconds as [Hp0 Hleb].
+      simpl. destruct (isU p) eqn:Hu.
+      ** assert (a <= a0)%a as Hle.
+         { destruct p; inversion Hu;simpl in Hleb;apply Z.leb_le in Hleb;solve_addr. }
+       iPureIntro. apply related_sts_a_weak_world with a0;auto.
+      ** assert (e <= a0)%a as Hle.
+         { destruct p; inversion Hu;simpl in Hleb;apply Z.leb_le in Hleb; try solve_addr. }
+         iPureIntro. apply related_sts_a_weak_world with a0;auto.
   - iModIntro. simpl. iIntros (W0 W1) "% HIW0".
     destruct g.
-    + by iApply interp_monotone_nm_nl.
+    + by iApply interp_monotone_nl.
     + (*Trick here: value relation leads to a contradiction if p0 is WL, since then its region cannot be permanent*)
       iDestruct ( writeLocalAllowed_valid_cap_implies with "Hvdst" ) as %Ha; eauto.
       rewrite Hstd in Ha. inversion Ha.
